ulib/FStar.Monotonic.Heap.fsti
@@ -52,9 +52,7 @@ val sel_tot: #a:Type0 -> #rel:preorder a -> h:heap -> r:mref a rel{h `contains` 
 
 val sel: #a:Type0 -> #rel:preorder a -> heap -> mref a rel -> GTot a
 
-let valid_upd (#a:Type0) (#rel:preorder a) (h:heap) (r:mref a rel) (x:a) = rel (sel h r) x
-
-val upd_tot: #a:Type0 -> #rel:preorder a -> h:heap -> r:mref a rel{h `contains` r} -> x:a{valid_upd h r x} -> Tot heap
+val upd_tot: #a:Type0 -> #rel:preorder a -> h:heap -> r:mref a rel{h `contains` r} -> x:a -> Tot heap
 
 val upd: #a:Type0 -> #rel:preorder a -> h:heap -> r:mref a rel -> x:a -> GTot heap
 
@@ -101,7 +99,7 @@ val lemma_distinct_addrs_distinct_preorders
 val lemma_distinct_addrs_distinct_mm
     (#a #b:Type0) (#rel1:preorder a) (#rel2: preorder b) (h:heap) (r1:mref a rel1) (r2:mref b rel2)
   :Lemma (requires (is_mm r1 =!= is_mm r2 /\ h `contains` r1 /\ h `contains` r2))
-          (ensures  (addr_of r1 <> addr_of r2))
+         (ensures  (addr_of r1 <> addr_of r2))
   [SMTPatT (h `contains` r1); SMTPatT (h `contains` r2)]
 
 (*
@@ -118,7 +116,7 @@ val lemma_distinct_addrs_unused
 val lemma_alloc (#a:Type0) (rel:preorder a) (h0:heap) (x:a) (mm:bool)
   :Lemma (requires True)
          (ensures  (let r, h1 = alloc rel h0 x mm in
-                    fresh r h0 h1 /\ valid_upd h0 r x /\ h1 == upd h0 r x /\ is_mm r = mm))
+                    fresh r h0 h1 /\ h1 == upd h0 r x /\ is_mm r = mm))
 	 [SMTPat (alloc rel h0 x mm)]
 
 val lemma_free_mm_sel
@@ -150,24 +148,24 @@ val lemma_free_mm_unused
  * AR: we can prove this lemma only if both the mreferences have same preorder
  *)
 val lemma_sel_same_addr (#a:Type0) (#rel:preorder a) (h:heap) (r1:mref a rel) (r2:mref a rel)
-  :Lemma (requires (h `contains` r1 /\ addr_of r1 = addr_of r2))
+  :Lemma (requires (h `contains` r1 /\ addr_of r1 == addr_of r2 /\ is_mm r1 == is_mm r2))
          (ensures  (h `contains` r2 /\ sel h r1 == sel h r2))
 	 [SMTPat (sel h r1); SMTPat (sel h r2)]
 
 val lemma_upd_same_addr (#a: Type0) (#rel: preorder a) (h: heap) (r1 r2: mref a rel) (x: a)
-  :Lemma (requires ((h `contains` r1 \/ h `contains` r2) /\ addr_of r1 = addr_of r2))
+  :Lemma (requires ((h `contains` r1 \/ h `contains` r2) /\ addr_of r1 == addr_of r2 /\ is_mm r1 == is_mm r2))
          (ensures (upd h r1 x == upd h r2 x))
          [SMTPat (upd h r1 x); SMTPat (upd h r2 x)]
 
  (*
   * AR: this is true only if the preorder is same, else r2 may not be contained in h
   *)
-val lemma_sel_upd1 (#a:Type0) (#rel:preorder a) (h:heap) (r1:mref a rel) (x:a{valid_upd h r1 x}) (r2:mref a rel)
-  :Lemma (requires (addr_of r1 = addr_of r2))
+val lemma_sel_upd1 (#a:Type0) (#rel:preorder a) (h:heap) (r1:mref a rel) (x:a) (r2:mref a rel)
+  :Lemma (requires (addr_of r1 = addr_of r2 /\ is_mm r1 == is_mm r2))
          (ensures  (sel (upd h r1 x) r2 == x))
          [SMTPat (sel (upd h r1 x) r2)]
 
-val lemma_sel_upd2 (#a:Type0) (#b:Type0) (#rel1:preorder a) (#rel2:preorder b) (h:heap) (r1:mref a rel1) (r2:mref b rel2) (x:b{valid_upd h r2 x})
+val lemma_sel_upd2 (#a:Type0) (#b:Type0) (#rel1:preorder a) (#rel2:preorder b) (h:heap) (r1:mref a rel1) (r2:mref b rel2) (x:b)
   :Lemma (requires (addr_of r1 <> addr_of r2))
          (ensures  (sel (upd h r2 x) r1 == sel h r1))
 	 [SMTPat (sel (upd h r2 x) r1)]
@@ -180,20 +178,20 @@ val lemma_in_dom_emp (#a:Type0) (#rel:preorder a) (r:mref a rel)
          (ensures  (r `unused_in` emp))
 	 [SMTPat (r `unused_in` emp)]
 
-val lemma_upd_contains (#a:Type0) (#rel:preorder a) (h:heap) (r:mref a rel) (x:a{valid_upd h r x})
+val lemma_upd_contains (#a:Type0) (#rel:preorder a) (h:heap) (r:mref a rel) (x:a)
   :Lemma (requires True)
          (ensures  ((upd h r x) `contains` r))
 	 [SMTPat ((upd h r x) `contains` r)]
 
 val lemma_well_typed_upd_contains
-  (#a:Type0) (#b:Type0) (#rel1:preorder a) (#rel2:preorder b) (h:heap) (r1:mref a rel1) (x:a{valid_upd h r1 x}) (r2:mref b rel2)
+  (#a:Type0) (#b:Type0) (#rel1:preorder a) (#rel2:preorder b) (h:heap) (r1:mref a rel1) (x:a) (r2:mref b rel2)
   :Lemma (requires (h `contains` r1))
          (ensures  (let h1 = upd h r1 x in
 	            h1 `contains` r2 <==> h `contains` r2))
 	 [SMTPat ((upd h r1 x) `contains` r2)]
 
 val lemma_unused_upd_contains
-  (#a:Type0) (#b:Type0) (#rel1:preorder a) (#rel2:preorder b) (h:heap) (r1:mref a rel1) (x:a{valid_upd h r1 x}) (r2:mref b rel2)
+  (#a:Type0) (#b:Type0) (#rel1:preorder a) (#rel2:preorder b) (h:heap) (r1:mref a rel1) (x:a) (r2:mref b rel2)
   :Lemma (requires (r1 `unused_in` h))
          (ensures  (let h1 = upd h r1 x in
 	            (h `contains` r2  ==> h1 `contains` r2) /\
@@ -201,32 +199,32 @@ val lemma_unused_upd_contains
 	 [SMTPat ((upd h r1 x) `contains` r2)]
 
 val lemma_upd_contains_different_addr
-  (#a:Type0) (#b:Type0) (#rel1:preorder a) (#rel2:preorder b) (h:heap) (r1:mref a rel1) (x:a{valid_upd h r1 x}) (r2:mref b rel2)
+  (#a:Type0) (#b:Type0) (#rel1:preorder a) (#rel2:preorder b) (h:heap) (r1:mref a rel1) (x:a) (r2:mref b rel2)
   :Lemma (requires (h `contains` r2 /\ addr_of r1 <> addr_of r2))
          (ensures  ((upd h r1 x) `contains` r2))
 	 [SMTPat ((upd h r1 x) `contains` r2)]
 
 val lemma_upd_unused
-  (#a:Type0) (#b:Type0) (#rel1:preorder a) (#rel2:preorder b) (h:heap) (r1:mref a rel1) (x:a{valid_upd h r1 x}) (r2:mref b rel2)
+  (#a:Type0) (#b:Type0) (#rel1:preorder a) (#rel2:preorder b) (h:heap) (r1:mref a rel1) (x:a) (r2:mref b rel2)
   :Lemma (requires True)
          (ensures  ((addr_of r1 <> addr_of r2 /\ r2 `unused_in` h) <==> r2 `unused_in` (upd h r1 x)))
 	 [SMTPat (r2 `unused_in` (upd h r1 x))]
 
-val lemma_contains_upd_modifies (#a:Type0) (#rel:preorder a) (h:heap) (r:mref a rel) (x:a{valid_upd h r x})
+val lemma_contains_upd_modifies (#a:Type0) (#rel:preorder a) (h:heap) (r:mref a rel) (x:a)
   :Lemma (requires (h `contains` r))
          (ensures  (modifies (S.singleton (addr_of r)) h (upd h r x)))
          [SMTPat (upd h r x)]
 
-val lemma_unused_upd_modifies (#a:Type0) (#rel:preorder a) (h:heap) (r:mref a rel) (x:a{valid_upd h r x})
+val lemma_unused_upd_modifies (#a:Type0) (#rel:preorder a) (h:heap) (r:mref a rel) (x:a)
   :Lemma (requires (r `unused_in` h))
          (ensures  (modifies (Set.singleton (addr_of r)) h (upd h r x)))
          [SMTPat (upd h r x); SMTPat (r `unused_in` h)]
 
 val upd_upd_same_mref
   (#a:Type) (#rel:preorder a) (h:heap) (r:mref a rel)
-  (x:a{valid_upd h r x}) (y:a{valid_upd (upd h r x) r y})
+  (x:a) (y:a)
   :Lemma (requires True)
-         (ensures  (valid_upd h r y /\ (upd (upd h r x) r y == upd h r y)))
+         (ensures  (upd (upd h r x) r y == upd h r y))
 	 [SMTPat (upd (upd h r x) r y)]
 
 val lemma_sel_equals_sel_tot_for_contained_refs
@@ -236,7 +234,7 @@ val lemma_sel_equals_sel_tot_for_contained_refs
 	 [SMTPat (sel_tot h r)]
 
 val lemma_upd_equals_upd_tot_for_contained_refs
-  (#a:Type0) (#rel:preorder a) (h:heap) (r:mref a rel{h `contains` r}) (x:a{valid_upd h r x})
+  (#a:Type0) (#rel:preorder a) (h:heap) (r:mref a rel{h `contains` r}) (x:a)
   :Lemma (requires True)
          (ensures  (upd_tot h r x == upd h r x))
 	 [SMTPat (upd_tot h r x)]
@@ -364,6 +362,3 @@ let upd_ref_of
   (ensures (aref_live_at h2 a t rel /\ upd h1 (ref_of h2 a t rel) x == upd h1 (gref_of a t rel) x))
   [SMTPat (upd h1 (ref_of h2 a t rel) x)]
 = ()
-
-(* Work around #1088 *)
-val _eof: unit
